LambdaS5/coq/LjsRulesCorrect.v
@@ -5,8 +5,8 @@ Require Import JsNumber.
 Require Import Utils.
 Require LjsSyntax LjsPrettyRules LjsPrettyInterm LjsStore LjsAuxiliary.
 Require EjsSyntax.
-Require JsSyntax JsPrettyRules JsPrettyInterm.
-Require Import EjsFromJs EjsToLjs.
+Require JsSyntax JsPrettyInterm JsPrettyRules.
+Require EjsFromJs EjsToLjs.
 Import ListNotations.
 Open Scope list_scope.
 Open Scope string_scope.
@@ -19,15 +19,20 @@ Include LjsPrettyRules.
 Include LjsPrettyInterm.
 Include LjsStore.
 Include LjsAuxiliary.
+Include LjsValues.
 End L.
 
-Module E := EjsSyntax.
+Module E.
+Include EjsSyntax.
+Include EjsFromJs.
+Include EjsToLjs.
+End E.
 
 Module J.
 Include JsSyntax.
 Include JsPreliminary.
-Include JsPrettyRules.
 Include JsPrettyInterm.
+Include JsPrettyRules.
 End J.
 
 Implicit Type A B : Type.
@@ -53,6 +58,9 @@ Implicit Type jr : J.res.
 Implicit Type jv : J.value.
 Implicit Type jptr : J.object_loc.
 Implicit Type jobj : J.object.
+Implicit Type jrv : J.resvalue.
+Implicit Type jt : J.stat.
+Implicit Type jref : J.ref.
 
 Definition object_bisim := J.object_loc -> L.object_ptr -> Prop.
 
@@ -137,48 +145,114 @@ Definition heaps_bisim BR jst st := forall jptr ptr jobj obj,
      L.object_binds st ptr obj ->
      object_related BR jobj obj.
 
-Definition js_literal_to_ljs jl := ejs_to_ljs (js_literal_to_ejs jl).
-Definition js_expr_to_ljs je := ejs_to_ljs (js_expr_to_ejs je).
+Definition js_literal_to_ljs jl := E.ejs_to_ljs (E.js_literal_to_ejs jl).
+Definition js_expr_to_ljs je := E.ejs_to_ljs (E.js_expr_to_ejs je).
+Definition js_stat_to_ljs jt := E.ejs_to_ljs (E.js_stat_to_ejs jt).
 
-Inductive res_related BR : J.res -> L.res -> Prop :=
-| res_related_normal_value : forall jv v,
+Inductive resvalue_related BR : J.resvalue -> L.value -> Prop :=
+| resvalue_related_value : forall jv v,
     value_related BR jv v ->
-    res_related BR (J.res_intro J.restype_normal (J.resvalue_value jv) J.label_empty) (L.res_value v)
+    resvalue_related BR (J.resvalue_value jv) v
 .
 
+Definition js_exn_object obj v := 
+    Heap.binds (L.object_properties_ obj) "%js-exn" 
+        (L.attributes_data_of (L.attributes_data_intro v false false false)).
+
+Inductive res_related BR jst st : J.res -> L.res -> Prop :=
+| res_related_normal : forall jrv v,
+    resvalue_related BR jrv v ->
+    res_related BR jst st (J.res_intro J.restype_normal jrv J.label_empty) (L.res_value v)
+| res_related_throw : forall jrv ptr obj v,
+    L.object_binds st ptr obj ->
+    js_exn_object obj v ->
+    res_related BR jst st (J.res_intro J.restype_throw jrv J.label_empty) 
+        (L.res_exception (L.value_object ptr))
+.
+
+(*
 Inductive out_related BR : J.out -> L.out -> Prop :=
 | out_related_ter : forall jst st jr r,
     res_related BR jr r ->
     out_related BR (J.out_ter jst jr) (L.out_ter st r)
 .
+*)
 
 Create HintDb js_ljs discriminated.
 
 Hint Constructors attributes_data_related : js_ljs.
-Hint Constructors attributes_accessor_related : js_ljs.
+Hint Constructors attributes_accessor_related : js_ljs. 
 Hint Constructors attributes_related : js_ljs.
 Hint Constructors value_related : js_ljs.
+Hint Constructors resvalue_related : js_ljs.
 Hint Constructors res_related : js_ljs.
-Hint Constructors out_related : js_ljs.
+(* Hint Constructors out_related : js_ljs. *)
 
 Hint Constructors J.red_expr : js_ljs.
+Hint Constructors J.red_stat : js_ljs.
+Hint Constructors J.red_spec : js_ljs.
 
-Definition concl_expr BR jst jc st c o je :=
-    exists jo,
-    J.red_expr jst jc (J.expr_basic je) jo /\ 
-    out_related BR jo o.
+Definition state_invariant BR jst jc c st :=
+    heaps_bisim BR jst st.
 
-Definition concl_stat BR jst jc st c o jt :=
-    exists jo,
-    J.red_stat jst jc (J.stat_basic jt) jo /\ 
-    out_related BR jo o.
+Definition concl_expr_value BR jst jc c st st' r je :=
+    exists jst' jr,
+    state_invariant BR jst' jc c st' /\
+    J.red_expr jst jc (J.expr_basic je) (J.out_ter jst' jr) /\ 
+    res_related BR jst' st' jr r.
 
-Lemma red_expr_literal_ok : forall jst jc st c o l BR, 
-    L.red_expr c st (L.expr_basic (js_literal_to_ljs l)) o ->
-    concl_expr BR jst jc st c o (J.expr_literal l).
+Definition concl_stat BR jst jc c st st' r jt :=
+    exists jst' jr,
+    state_invariant BR jst' jc c st' /\
+    J.red_stat jst jc (J.stat_basic jt) (J.out_ter jst' jr) /\ 
+    res_related BR jst' st' jr r.
+
+(*
+Definition concl_spec {A : Type} BR jst jc c st st' r js (P : A -> Prop) :=
+    exists jst',
+    state_invariant BR jst' jc c st' /\ 
+    ((exists x, J.red_spec jst jc js (J.specret_val jst' x) /\ P x) \/
+     (exists jr, 
+        J.red_spec jst jc js (@J.specret_out A (J.out_ter jst' jr)) /\ 
+        res_related BR jst' st' jr r)).
+*)
+
+Definition concl_spec {A : Type} BR jst jc c st st' r js (P : A -> Prop) :=
+    exists jst',
+    state_invariant BR jst' jc c st' /\ 
+    ((exists x, J.red_spec jst jc js (J.specret_val jst' x) /\ P x) \/
+     (exists jr, 
+        J.red_spec jst jc js (@J.specret_out A (J.out_ter jst' jr)) /\ 
+        J.abort (J.out_ter jst' jr) /\
+        res_related BR jst' st' jr r)).
+
+Definition concl_expr_getvalue BR jst jc c st st' r je :=
+    concl_spec BR jst jc c st st' r (J.spec_expr_get_value je) 
+       (fun jv => exists v, r = L.res_value v /\ value_related BR jv v).
+
+(*
+Definition ih_expr je := forall BR jst jc c st st' r, 
+    state_invariant BR jst jc c st ->
+    L.red_expr c st (L.expr_basic (js_expr_to_ljs je)) (L.out_ter st' r) ->
+    concl_expr BR jst jc c st st' r je.
+*)
+Definition ih_expr je := forall BR jst jc c st st' r, 
+    state_invariant BR jst jc c st ->
+    L.red_expr c st (L.expr_basic (js_expr_to_ljs je)) (L.out_ter st' r) ->
+    concl_expr_getvalue BR jst jc c st st' r je.
+
+Definition ih_stat jt := forall BR jst jc c st st' r, 
+    state_invariant BR jst jc c st ->
+    L.red_expr c st (L.expr_basic (js_stat_to_ljs jt)) (L.out_ter st' r) ->
+    concl_stat BR jst jc c st st' r jt.
+
+Lemma red_expr_literal_ok : forall jst jc c st st' r l BR, 
+    state_invariant BR jst jc c st ->
+    L.red_expr c st (L.expr_basic (js_literal_to_ljs l)) (L.out_ter st' r) ->
+    concl_expr_value BR jst jc c st st' r (J.expr_literal l).
 Proof.
-    introv lred.
-    destruct l as [ | [ | ] | | ]; inverts lred; eexists; eauto with js_ljs.
+    introv Hinv Hlred.
+    destruct l as [ | [ | ] | | ]; inverts Hlred; eexists; jauto_set; eauto with js_ljs.
 Qed.
 
 Ltac inv_internal_ljs :=
@@ -191,22 +265,148 @@ Ltac inv_internal_ljs :=
     end
 .
 
-Lemma red_stat_expr_ok : forall jst jc st c o je BR, 
-    (forall BR jst jc st c o, L.red_expr c st (L.expr_basic (js_expr_to_ljs je)) o ->
-      concl_expr BR jst jc st c o je) ->
-    L.red_expr c st (L.expr_basic (js_expr_to_ljs je)) o ->
-    concl_stat BR jst jc st c o (J.stat_expr je).
+Ltac inv_res_related :=
+    match goal with
+    | H : res_related _ _ _ |- _ => inverts H
+    end.
+
+Ltac inv_resvalue_related :=
+    match goal with
+    | H : resvalue_related _ _ _ |- _ => inverts H
+    end.
+
+Ltac unfold_concl := unfold concl_expr_value, concl_expr_getvalue, concl_stat, concl_spec in *.
+
+Ltac jauto_js := repeat (jauto_set; eauto with js_ljs).
+
+Hint Extern 10 => match goal with 
+    | H : J.abort_intercepted_stat _ |- _ => solve [inverts H]
+    end : js_ljs. 
+
+Lemma red_stat_expr_ok : forall jst jc c st st' r je BR, 
+    ih_expr je ->
+    state_invariant BR jst jc c st ->
+    L.red_expr c st (L.expr_basic (js_expr_to_ljs je)) (L.out_ter st' r) ->
+    concl_stat BR jst jc c st st' r (J.stat_expr je).
 Proof.
-    introv IH lred.
-    specializes IH lred.
-    destruct IH.
-    eexists x.
-    destruct H.
-    splits.    
-    eapply J.red_stat_expr.
-    eapply J.red_spec_expr_get_value.
-    eassumption.
+    introv IH Hinv Hlred.
+    specializes IH Hinv Hlred.
+    unfold_concl.
+    destruct IH as (jst'&Hinv'&[|]). (* TODO better tactics *)
+    jauto_js.
+    substs.
+    jauto_js.
+    jauto_js.
+Qed.
+(*
+Lemma red_spec_get_value_ok : forall jst jc c st st' r je BR, 
+    ih_expr je ->
+    state_invariant BR jst jc c st ->
+    L.red_expr c st (L.expr_basic (js_expr_to_ljs je)) (L.out_ter st' r) ->
+    concl_spec BR jst jc c st st' r (J.spec_expr_get_value je) 
+       (fun jv => exists v, r = L.res_value v /\ value_related BR jv v).
+Proof.
+    introv IHe Hinv Hlred.
+    specializes IHe Hinv Hlred.
+    unfold_concl.
+    jauto_js. 
+    inverts H1. inverts H2. (* TODO *)
+    left.
+    jauto_js.
+Qed.
+*)
+(* TODO
+Lemma ljs_to_bool_lemma : forall BR jst jc c st st' r jv v loc v1,
+    state_invariant BR jst jc c st ->
+    value_related BR jv v -> 
+    L.id_binds c "%ToBoolean" loc ->
+    L.value_binds st loc v1 ->
+    L.red_expr c st (L.expr_app_2 v1 [v] nil) (L.out_ter st' r) ->
+    st = st' /\
+    exists b,
+    r = L.res_value (L.bool_to_value b) /\
+    J.red_expr jst jc (J.spec_to_boolean jv) 
+        (J.out_ter jst (J.res_val (J.value_prim (J.prim_bool b)))).
+Proof.
 Admitted.
+*)
+
+Lemma red_spec_to_boolean_ok : forall jst jc c st st' r je BR, 
+    ih_expr je ->
+    state_invariant BR jst jc c st ->
+    L.red_expr c st (L.expr_basic (E.to_bool (js_expr_to_ljs je))) (L.out_ter st' r) ->
+    concl_spec BR jst jc c st st' r (J.spec_expr_get_value_conv J.spec_to_boolean je) 
+       (fun jv => exists b, jv = J.value_prim (J.prim_bool b) /\ 
+           r = L.res_value (L.bool_to_value b)).
+Proof.
+    introv IHe Hinv Hlred.
+    inverts Hlred.
+Admitted.
+
+Lemma res_related_abort : forall BR jst jst' st jr r,
+    res_related BR jst st jr r ->
+    J.abort (J.out_ter jst' jr) ->
+    L.res_is_control r.
+Proof.
+    introv Hrel Hab.
+    inverts Hrel.
+    inverts Hab. unfold J.res_is_normal in *. simpls. tryfalse.
+    eapply L.res_is_control_exception.
+Qed.
+
+Lemma red_stat_if_ok : forall jst jc c st st' r je jt1 jt2 BR, 
+    ih_expr je ->
+    ih_stat jt1 ->
+    ih_stat jt2 ->
+    state_invariant BR jst jc c st ->
+    L.red_expr c st (L.expr_basic (js_stat_to_ljs (J.stat_if je jt1 (Some jt2)))) (L.out_ter st' r) ->
+    concl_stat BR jst jc c st st' r (J.stat_if je jt1 (Some jt2)).
+Proof.
+    introv IHe IHt1 IHt2 Hinv Hlred.
+    inverts Hlred.
+    destruct o.
+    inverts H6.
+    forwards Hh : red_spec_to_boolean_ok IHe Hinv H5.
+    unfold concl_spec in Hh.
+    destruct Hh as (jst'&Hinv'&[|]). (* TODO better tactics *)
+    jauto_set.
+    substs.
+    destruct x0.
+    (* true *) 
+    inverts H6.
+    specializes IHt1 Hinv' H8.
+    unfold concl_stat in *.
+    jauto_js.
+    inverts H3. inverts H1.
+    (* false *)
+    inverts H6.
+    specializes IHt2 Hinv' H8.
+    unfold concl_stat in *.
+    jauto_js.
+    inverts H3. inverts H1.
+    (* abort *)
+    jauto_set. 
+    forwards Hab : res_related_abort H1 H0.
+    inverts H6.
+    inverts Hab. 
+    inverts Hab. 
+    unfold concl_stat.
+    jauto_js.
+Qed.
+
+Lemma red_stat_throw_ok : forall jst jc c st st' r je BR,
+    ih_expr je ->
+    state_invariant BR jst jc c st ->
+    L.red_expr c st (L.expr_basic (js_stat_to_ljs (J.stat_throw je))) (L.out_ter st' r) ->
+    concl_stat BR jst jc c st st' r (J.stat_throw je).
+Proof.
+    introv IHe Hinv Hlred.
+    inverts Hlred.
+    inverts H0.
+Admitted. (* TODO lemmas, tactics needed! *)
+
+    
+    
 
 (*
 
@@ -217,38 +417,4 @@ Lemma red_identifier_ok : forall jst jc st c o i BR,
     J.red_expr jst jc (J.expr_basic (J.expr_identifier i)) jo /\
     out_related BR jo o.
 Proof.
-    introv Bisim lred.
-    inverts lred.
-
-    introv jred lred.
-    inverts jred; inverts lred; tryfalse.
-    inv_internal_ljs.
-    inv_internal_ljs.
-    inv_internal_ljs.
-    inv_internal_ljs.
-    inv_internal_ljs.
-    inv_internal_ljs.
-    inv_internal_ljs.
-    inv_internal_ljs.
-    inv_internal_ljs.
-    inv_internal_ljs.
-    inv_internal_ljs.
-    inv_internal_ljs.
-    inv_internal_ljs.
-    inv_internal_ljs.
-    inv_internal_ljs.
-    inv_internal_ljs.
-    inv_internal_ljs.
-    inv_internal_ljs.
-
-
-    repeat inv_internal_ljs.
-    inverts H7; tryfalse.
-    inverts H8; tryfalse.
-    inverts H11; tryfalse.
-    inverts H12; tryfalse.
-
-    inverts H0; tryfalse.
-    inverts H3; tryfalse.
-
 *)
