LambdaS5/coq/Utils.v
@@ -97,3 +97,50 @@ Tactic Notation "injects" :=
     | H : _ = _ |- _ => injects H
     end.
 
+(* TODO move to TLC *)
+Global Instance Exists_decidable : 
+    forall `(l : list A) P (HD : forall a, Decidable (P a)), Decidable (Exists P l).
+Proof.
+    introv HD.
+    applys decidable_make (exists_st (fun a => decide (P a)) l).
+    induction l as [ | a l]; unfolds exists_st; simpl.
+    fold_bool; rew_reflect. eauto using Exists_nil_inv. 
+    rew_refl.
+    rewrite IHl.
+    remember (isTrue (P a)) as b1 eqn: Eq1.
+    destruct b1; rew_bool; fold_bool. 
+    rew_refl in *.
+    apply~ Exists_here.
+    remember (isTrue (Exists P l)) as b2 eqn: Eq2.
+    destruct b2; fold_bool.
+    rew_reflect in *.
+    apply~ Exists_next.
+    rew_reflect in *.
+    intro.
+    inverts~ H.
+Defined.
+
+(* TODO move to utilities *)
+
+Inductive Has_dupes {A : Type} : list A -> Prop :=
+    | Has_dupes_here : forall a l, Exists (fun b => a = b) l -> Has_dupes (a :: l)
+    | Has_dupes_next : forall a l, Has_dupes l -> Has_dupes (a :: l).
+
+Fixpoint has_dupes `{c : Comparable A} (l : list A) := 
+    match l with
+    | a :: l' => exists_st (fun b => decide (a = b)) l' || has_dupes l'
+    | nil => false
+    end.
+
+Global Instance Has_dupes_decidable : forall `(l : list A) `(c : Comparable A),
+    Decidable (Has_dupes l).
+Proof.
+    intros.
+    applys decidable_make (has_dupes l).
+    induction l as [ | a l]; unfold has_dupes; simpl.
+    fold_bool; rew_reflect. intro. inverts H.
+    fold has_dupes.
+    rewrite IHl.
+    skip. (* TODO *)
+Defined.
+
